Implemented Map in list to prove some of the assumptions, the registers typing is now in MapList as opposed to TreeMap

DEX_I/Annotated.v
@@ -32,12 +32,12 @@ Definition well_formed_lookupswitch m := forall pc reg l size i o1 o2,
   instructionAt m pc = Some (DEX_SparseSwitch reg size l) ->
   In (i, o1) l -> In (i, o2) l -> o1=o2.
 
-Module VarMap := BinNatMap.
-Definition TypeRegisters := VarMap.t L.t(* focus on DEX I'*).
+Module VarMap := MapList.
+Definition TypeRegisters := MapList.t L.t(* focus on DEX I'*).
 
-Definition update_op (rt:TypeRegisters) (key:VarMap.key) (k:option L.t(*'*)) :=
+Definition update_op (rt:TypeRegisters) (key:MapList.key) (k:option L.t(*'*)) :=
   match k with
-    | Some v => BinNatMap.update _ rt key v
+    | Some v => MapList.update rt key v
     | None => rt
   end.
 
@@ -88,45 +88,49 @@ Qed.
 Fixpoint make_rt_from_lvt_rec (s:DEX_sign) (p:list DEX_Reg) (valid_regs:list DEX_Reg) (default:L.t) {struct valid_regs} : TypeRegisters:=
   match valid_regs with
     | r::t => 
-        VarMap.update _ (make_rt_from_lvt_rec s p t default) r (if In_test r p then DEX_lvt s r else default)
-    | nil => VarMap.empty L.t
+        MapList.update (make_rt_from_lvt_rec s p t default) r (if In_test r p then DEX_lvt s r else default)
+    | nil => MapList.empty L.t
   end.
 
+Lemma make_rt_from_lvt_prop4 : forall s v p d r, In r (MapList.dom (make_rt_from_lvt_rec s p v d)) -> In r v.
+Proof.
+  induction v; intros.
+  inversion H.
+  simpl in H.
+  unfold MapList.dom in H. 
+
 Lemma make_rt_from_lvt_prop1 : forall s v p d r, 
-  (forall k, In r p -> Some k = VarMap.get _ (make_rt_from_lvt_rec s p v d) r -> k = (DEX_lvt s r)).
+  (forall k, In r p -> Some k = MapList.get (make_rt_from_lvt_rec s p v d) r -> k = (DEX_lvt s r)).
 Proof.
   intros.
   induction v.
-  intros. simpl in H0. rewrite VarMap.get_empty in H0. inversion H0.
-  intros.
-  generalize (Neq_spec a r); intros Heq.
-  destruct (Neq a r). subst.
+  inversion H0.
   simpl in H0. 
-  apply In_In_test in H. rewrite H in H0.
-  rewrite VarMap.get_update1 in H0; auto. inversion H0; auto.
-  simpl in H0.
+  generalize (Neq_spec a r); destruct (Neq a r) eqn:Heq; intros.
+  apply In_In_test in H. subst. rewrite H in H0.
+  rewrite MapList.get_update1 in H0; auto. inversion H0; auto.
   destruct (In_test a p).
-  rewrite VarMap.get_update2 in H0; auto.
-  rewrite VarMap.get_update2 in H0; auto.
+  rewrite MapList.get_update2 in H0; auto.
+  rewrite MapList.get_update2 in H0; auto.
 Qed.
 
 Lemma make_rt_from_lvt_prop2 : forall s p v d r,
-  In r v -> ~In r p -> Some d = VarMap.get _ (make_rt_from_lvt_rec s p v d) r.
+  In r v -> ~In r p -> Some d = MapList.get (make_rt_from_lvt_rec s p v d) r.
 Proof.
   intros.
   induction v.
   inversion H.
   inversion H.
   subst. simpl. apply not_In_In_test in H0. rewrite H0.
-  rewrite VarMap.get_update1; auto.
+  rewrite MapList.get_update1; auto.
   apply IHv in H1.
   simpl. 
   generalize (Neq_spec a r); intros Heq.
   destruct (Neq a r). subst. 
-  apply not_In_In_test in H0. rewrite H0. rewrite VarMap.get_update1; auto.
+  apply not_In_In_test in H0. rewrite H0. rewrite MapList.get_update1; auto.
   destruct (In_test a p).
-  subst; rewrite VarMap.get_update2; auto.
-  rewrite VarMap.get_update2; auto.
+  subst; rewrite MapList.get_update2; auto.
+  rewrite MapList.get_update2; auto.
 Qed.
 
 Fixpoint eq_set_r_test (regs dom1 dom2:@list DEX_PC) : bool :=
@@ -211,12 +215,12 @@ Proof.
 Qed.
  
 
-Inductive eq_rt (rt1 rt2:VarMap.t L.t) : Prop :=
-  forall_rt : eq_set (VarMap.dom L.t rt1) (VarMap.dom L.t rt2) ->
-    (forall r, In r (VarMap.dom L.t rt1) -> In r (VarMap.dom L.t rt2) ->
-    forall k1 k2, Some k1 = VarMap.get _ rt1 r -> Some k2 = VarMap.get _ rt2 r -> k1 = k2) -> eq_rt rt1 rt2.
+Inductive eq_rt (rt1 rt2:MapList.t L.t) : Prop :=
+  forall_rt : eq_set (MapList.dom rt1) (MapList.dom rt2) ->
+    (forall r, In r (MapList.dom rt1) -> In r (MapList.dom rt2) ->
+    forall k1 k2, Some k1 = MapList.get rt1 r -> Some k2 = MapList.get rt2 r -> k1 = k2) -> eq_rt rt1 rt2.
 
-Lemma eq_rt_refl : reflexive (@VarMap.t L.t) eq_rt.
+Lemma eq_rt_refl : reflexive (@MapList.t L.t) eq_rt.
 Proof.
   unfold reflexive.
   constructor; intros. 
@@ -224,7 +228,7 @@ Proof.
   congruence.
 Qed.
 
-Lemma eq_rt_sym : symmetric (@VarMap.t L.t) eq_rt.
+Lemma eq_rt_sym : symmetric (@MapList.t L.t) eq_rt.
 Proof.
   unfold symmetric.
   constructor; intros;
@@ -233,17 +237,17 @@ Proof.
   apply H5 with (k1:=k2) (k2:=k1) in H1; auto.
 Qed.
 
-Lemma eq_rt_trans : transitive (@VarMap.t L.t) eq_rt.
+Lemma eq_rt_trans : transitive (@MapList.t L.t) eq_rt.
 Proof.
   unfold transitive.
   constructor; intros;
   inversion H; inversion H0.
-    apply eq_set_trans with (x:=VarMap.dom L.t x) (y:=VarMap.dom L.t y) (z:=VarMap.dom L.t z); auto.
+    apply eq_set_trans with (x:=MapList.dom x) (y:=MapList.dom y) (z:=MapList.dom z); auto.
   specialize H6 with (r:=r); specialize H8 with (r:=r).
   assert (H2':=H2).
   rewrite <- H7 in H2.
-  assert (exists ky, Some ky = VarMap.get L.t y r).
-    apply VarMap.in_dom_get_some in H2. destruct (VarMap.get L.t y r).
+  assert (exists ky, Some ky = MapList.get y r).
+    apply MapList.in_dom_get_some in H2. destruct (MapList.get y r).
     exists t; auto. elim H2; auto.
   destruct H9.
   specialize H6 with (1:=H1) (2:=H2) (3:=H3) (4:=H9) (k1:=k1) (k2:=x0);
@@ -252,634 +256,32 @@ Proof.
 Qed.
 
 Lemma eq_rt_get : forall rt1 rt2 r, eq_rt (rt1) (rt2) -> 
-  In r (VarMap.dom L.t rt1) -> In r (VarMap.dom L.t rt2) -> 
-  VarMap.get L.t rt1 r = VarMap.get L.t rt2 r.
+  In r (MapList.dom rt1) -> In r (MapList.dom rt2) -> 
+  MapList.get rt1 r = MapList.get rt2 r.
 Proof.
   intros.
   inversion H.
   specialize H3 with (1:=H0) (2:=H1).
-  destruct (VarMap.get L.t rt1 r) eqn:Hrt1; destruct (VarMap.get L.t rt2 r) eqn:Hrt2; auto.
+  destruct (MapList.get rt1 r) eqn:Hrt1; destruct (MapList.get rt2 r) eqn:Hrt2; auto.
   assert (t = t0). apply H3 with (k1:=t) (k2:=t0); auto. 
   congruence.
-  apply VarMap.in_dom_get_some in H1; apply False_ind; auto.
-  apply VarMap.in_dom_get_some in H0; apply False_ind; auto.
+  apply MapList.in_dom_get_some in H1; apply False_ind; auto.
+  apply MapList.in_dom_get_some in H0; apply False_ind; auto.
 Qed.
 
-Lemma fold_rec_subst_leaf_1 : forall p v n acc, (length (fold_rec L.t (list BinNatMap_Base.key)
-        (fun (p0 : BinMap_Base.key) (_ : L.t) (b : list BinNatMap_Base.key) => N.pos p0 :: b)
-        (subst_leaf (option L.t) None p (Some v)) n acc)) = S (length acc)%nat.
+Lemma dom_length_update_nodup : forall m a v, ~In a (MapList.dom m) ->  
+  length (MapList.dom (MapList.update m a v)) = S (length (@MapList.dom L.t m)).
 Proof.
-  induction p; auto; intros; try (simpl; apply IHp).
+  induction m; intros; auto.
+  simpl in *. 
+  generalize (Neq_spec a0 (fst a)); destruct (Neq a0 (fst a)) eqn:Heq; intros.
+  apply False_ind; auto.
+  simpl. rewrite IHm; auto.
 Qed.
 
-Lemma fold_subst_leaf_1 : forall p v, length (BinMap_Base.fold L.t (list BinNatMap_Base.key)
-        (fun (p0 : BinMap_Base.key) (_ : L.t) (b : list BinNatMap_Base.key) => N.pos p0 :: b)
-        (subst_leaf (option L.t) None p (Some v)) nil) = 1%nat.
-Proof.
-  unfold BinMap_Base.fold. unfold fold. intros.
-  apply fold_rec_subst_leaf_1 with (p:=p) (v:=v) (n:=1).
-Qed.
-
-Lemma fold_rec_unroll_None : forall (A B:Type) f t1 t2 n acc,
-  fold_rec A B f (node (option A) (@None A) t1 t2) n acc =
-    fold_rec A B f t2 n~1 (fold_rec A B f t1 n~0 acc).
-Proof. auto. Qed.
-
-Lemma fold_rec_unroll_Some : forall (A B:Type) a f t1 t2 n acc,
-  fold_rec A B f (node (option A) (Some a) t1 t2) n acc =
-    fold_rec A B f t2 n~1 (f (inv_pos n 1) a (fold_rec A B f t1 n~0 acc)).
-Proof. auto. Qed.
-
-Lemma modify_tree_unroll : forall (A:Type) (bot:option A) p a t1 t2 f,
-  modify_tree (option A) bot (node (option A) a t1 t2) p f =
-   match p with
-      | p'~1 => node _ a t1 (modify_tree _ bot t2 p' f)
-      | p'~0 => node _ a (modify_tree _ bot t1 p' f) t2
-      | 1 => node _ (f a) t1 t2
-      end.
-Proof. auto. Qed.
- 
-Lemma length_fold_rec_split : forall t2 n acc,
-  length
-(fold_rec L.t (list BinNatMap_Base.key)
-   (fun (p0 : BinMap_Base.key) (_ : L.t) (b : list BinNatMap_Base.key) =>
-    N.pos p0 :: b)
-   (t2) n acc) = (length
-(fold_rec L.t (list BinNatMap_Base.key)
-   (fun (p0 : BinMap_Base.key) (_ : L.t) (b : list BinNatMap_Base.key) =>
-    N.pos p0 :: b)
-   (t2) n nil ) + length (acc))%nat.
-Proof.
-  induction t2; auto; intros.
-  destruct a.
-  (* a is Some *)
-  rewrite fold_rec_unroll_Some.
-  rewrite IHt2_2.
-  rewrite fold_rec_unroll_Some.
-  replace (length
- (fold_rec L.t (list BinNatMap_Base.key)
-    (fun (p0 : BinMap_Base.key) (_ : L.t) (b : list BinNatMap_Base.key) =>
-     N.pos p0 :: b) t2_2 n~1
-    (N.pos (inv_pos n 1)
-     :: fold_rec L.t (list BinNatMap_Base.key)
-          (fun (p0 : BinMap_Base.key) (_ : L.t) (b : list BinNatMap_Base.key)
-           => N.pos p0 :: b) t2_1 n~0 nil))) with
-    (length
- (fold_rec L.t (list BinNatMap_Base.key)
-    (fun (p0 : BinMap_Base.key) (_ : L.t) (b : list BinNatMap_Base.key) =>
-     N.pos p0 :: b) t2_2 n~1 nil) + 
-    length
- (N.pos (inv_pos n 1)
-     :: fold_rec L.t (list BinNatMap_Base.key)
-          (fun (p0 : BinMap_Base.key) (_ : L.t) (b : list BinNatMap_Base.key)
-           => N.pos p0 :: b) t2_1 n~0 nil))%nat; auto.
-  simpl.
-  rewrite IHt2_1. rewrite <- plus_assoc. auto.
-  (* a is None *)
-  rewrite fold_rec_unroll_None. 
-  rewrite IHt2_2. 
-  rewrite fold_rec_unroll_None. 
-  replace (length (fold_rec L.t (list BinNatMap_Base.key)
-    (fun (p0 : BinMap_Base.key) (_ : L.t) (b : list BinNatMap_Base.key) =>
-     N.pos p0 :: b) t2_2 n~1
-    (fold_rec L.t (list BinNatMap_Base.key)
-       (fun (p0 : BinMap_Base.key) (_ : L.t) (b : list BinNatMap_Base.key) =>
-        N.pos p0 :: b) t2_1 n~0 nil)))
-  with ((length (fold_rec L.t (list BinNatMap_Base.key)
-    (fun (p0 : BinMap_Base.key) (_ : L.t) (b : list BinNatMap_Base.key) =>
-     N.pos p0 :: b) t2_2 n~1 nil) + 
-      length 
-        (fold_rec L.t (list BinNatMap_Base.key)
-       (fun (p0 : BinMap_Base.key) (_ : L.t) (b : list BinNatMap_Base.key) =>
-        N.pos p0 :: b) t2_1 n~0 nil))%nat ); auto.
-  rewrite IHt2_1. apply Nat.add_assoc.
-  Qed. 
-
-(*Lemma length_modify_tree_S : forall t2 p n v acc, length
-(fold_rec L.t (list BinNatMap_Base.key)
-   (fun (p0 : BinMap_Base.key) (_ : L.t) (b : list BinNatMap_Base.key) =>
-    N.pos p0 :: b)
-   (modify_tree (option L.t) None t2 p (fun _ : option L.t => Some v)) n acc) = 
-S (length
-(fold_rec L.t (list BinNatMap_Base.key)
-   (fun (p0 : BinMap_Base.key) (_ : L.t) (b : list BinNatMap_Base.key) =>
-    N.pos p0 :: b) t2 n acc)).
-Proof.
-  induction t2; auto; intros.
-  simpl. rewrite fold_rec_subst_leaf_1; auto.
-  rewrite modify_tree_unroll.
-  destruct p. destruct a.
-  rewrite fold_rec_unroll_Some. 
-  rewrite length_fold_rec_split. rewrite IHt2_2.
-  rewrite fold_rec_unroll_Some with (t1:=t2_1) (t2:=t2_2).
-  rewrite length_fold_rec_split with (t2:=t2_2) (acc:=(N.pos (inv_pos n 1)
-       :: fold_rec L.t (list BinNatMap_Base.key)
-            (fun (p0 : BinMap_Base.key) (_ : L.t)
-               (b : list BinNatMap_Base.key) => N.pos p0 :: b) t2_1 n~0 acc)).
-  rewrite plus_Sn_m; auto.
-  rewrite fold_rec_unroll_None.
-  rewrite length_fold_rec_split. rewrite IHt2_2.
-  rewrite fold_rec_unroll_None.
-  rewrite length_fold_rec_split with (acc:= (fold_rec L.t (list BinNatMap_Base.key)
-         (fun (p0 : BinMap_Base.key) (_ : L.t) (b : list BinNatMap_Base.key)
-          => N.pos p0 :: b) t2_1 n~0 acc)).
-  rewrite plus_Sn_m; auto.
-  destruct a.
-  rewrite fold_rec_unroll_Some. 
-  rewrite length_fold_rec_split. simpl. rewrite IHt2_1.
-  rewrite length_fold_rec_split with (t2:=t2_2) (acc:=(N.pos (inv_pos n 1)
-       :: fold_rec L.t (list BinNatMap_Base.key)
-            (fun (p0 : BinMap_Base.key) (_ : L.t)
-               (b : list BinNatMap_Base.key) => N.pos p0 :: b) t2_1 n~0 acc)).
-  simpl. omega.
-  rewrite fold_rec_unroll_None.
-  rewrite length_fold_rec_split. simpl. rewrite IHt2_1.
-  rewrite length_fold_rec_split with (acc:= (fold_rec L.t (list BinNatMap_Base.key)
-         (fun (p0 : BinMap_Base.key) (_ : L.t) (b : list BinNatMap_Base.key)
-          => N.pos p0 :: b) t2_1 n~0 acc)).
-  omega.
-  destruct a.
-  rewrite ?fold_rec_unroll_Some.
-  admit.
-  rewrite ?fold_rec_unroll_Some.
-  rewrite ?fold_rec_unroll_None.
-  rewrite length_fold_rec_split.
-(*     simpl.  *)
-  rewrite length_fold_rec_split with (t2:=t2_2) (acc:= (fold_rec L.t (list BinNatMap_Base.key)
-         (fun (p0 : BinMap_Base.key) (_ : L.t) (b : list BinNatMap_Base.key)
-          => N.pos p0 :: b) t2_1 n~0 acc)).
-  simpl. omega.
-Admitted.*)
-
-Lemma L1_aux : forall l1 l2 x, In x (fold_right (fun (pa : positive * L.t) (b0 : list N) =>
-      let (p0, _) := pa in N.pos p0 :: b0) (x::l1) (l2)).
-Proof.
-  induction l1; induction l2; intros; simpl; auto.
-  destruct a; apply in_cons; apply IHl2.
-  destruct a0; apply in_cons; apply IHl2.
-Qed.
-
-Lemma L2_aux : forall l1 l2 x, In x l1 ->
-  In x (fold_right (fun (pa : positive * L.t) (b0 : list N) =>
-      let (p0, _) := pa in N.pos p0 :: b0) (l1) (l2)).
-Proof.
-  induction l1; induction l2; intros; simpl; auto.
-  destruct a; apply in_cons; apply IHl2; auto.
-  destruct a0; apply in_cons; apply IHl2; auto.
-Qed.
- 
-Lemma L3_aux : forall (l1:list N) (l2:list (positive*L.t)) (x:positive), 
-  (exists a, In (x,a) l2) ->
-  In (N.pos x) (fold_right (fun (pa : positive * L.t) (b0 : list N) =>
-      let (p0, _) := pa in N.pos p0 :: b0) (l1) (l2)).
-Proof.
-  induction l1; induction l2; intros; simpl. inversion H. inversion H0.
-  destruct H. destruct a. inversion H.
-  inversion H0; subst. apply in_eq.
-  apply in_cons. apply IHl2; auto.
-  exists x0; auto.
-  destruct H. inversion H.
-  destruct a0. destruct H; inversion H. inversion H0.
-  subst; apply in_eq.
-  apply in_cons; apply IHl2; auto. exists x0; auto.
-Qed.
-
-Lemma L3_aux' : forall (x:positive) (l:list (positive*L.t)), 
-  In (N.pos x) (fold_right (fun (pa : positive * L.t) (b0 : list N) =>
-      let (p0, _) := pa in N.pos p0 :: b0) nil (l))
-  ->  (exists a, In (x,a) l).
-Proof.
-  intros until l.
-  rewrite <- fold_right_eq2 with (f1:=(fun (pa:prod positive L.t) (b0:list N) => Npos (fst pa)::b0)).
-    rewrite in_fold_cons; intros.
-    destruct (in_map_inv _ _ _ _ _ H).
-    destruct x0; simpl in *; intuition; subst; eauto.
-    inversion H1; subst; eauto.
-    destruct a; simpl; auto.
-Qed.
- 
-Lemma L1 : forall t1 t2 v acc, In 1%N
-  (fold_rec L.t (list BinNatMap_Base.key)
-    (fun (p : BinMap_Base.key) (_ : L.t) (b : list BinNatMap_Base.key) =>
-    N.pos p :: b) (node (option L.t) (Some v) t1 t2) 1 acc).
-Proof.
-  intros; simpl.
-  rewrite <- fold_rec_prop with (l:=nil) (b1:=1%N
-    :: fold_rec L.t (list BinNatMap_Base.key)
-         (fun (p : BinMap_Base.key) (_ : L.t) (b : list BinNatMap_Base.key) =>
-          N.pos p :: b) t1 2 acc); auto.
-  apply L1_aux.
-Qed.
-
-Variable length_modify_tree_S : forall t2 p n v acc,
-(*   (~In (N.pos p) (fold L.t (list BinNatMap_Base.key)
-            (fun (p : BinMap_Base.key) (_ : L.t) (b : list BinNatMap_Base.key) =>
-             N.pos p :: b) t2 nil)) -> *)  
-length
-  (fold_rec L.t (list BinNatMap_Base.key)
-    (fun (p0 : BinMap_Base.key) (_ : L.t) (b : list BinNatMap_Base.key) =>
-      N.pos p0 :: b)
-    (modify_tree (option L.t) None t2 p (fun _ : option L.t => Some v)) n acc) = 
-  S (length
-    (fold_rec L.t (list BinNatMap_Base.key)
-    (fun (p0 : BinMap_Base.key) (_ : L.t) (b : list BinNatMap_Base.key) =>
-      N.pos p0 :: b) t2 n acc)).
-(*
-Lemma length_modify_tree_S : forall t2 p n v acc, 
-   (~In (N.pos p) (fold L.t (list BinNatMap_Base.key)
-            (fun (p : BinMap_Base.key) (_ : L.t) (b : list BinNatMap_Base.key) =>
-             N.pos p :: b) t2 nil)) ->  
-length
-  (fold_rec L.t (list BinNatMap_Base.key)
-    (fun (p0 : BinMap_Base.key) (_ : L.t) (b : list BinNatMap_Base.key) =>
-      N.pos p0 :: b)
-    (modify_tree (option L.t) None t2 p (fun _ : option L.t => Some v)) n acc) = 
-  S (length
-    (fold_rec L.t (list BinNatMap_Base.key)
-    (fun (p0 : BinMap_Base.key) (_ : L.t) (b : list BinNatMap_Base.key) =>
-      N.pos p0 :: b) t2 n acc)).
-Proof.
-  (* old proof *)
-  induction t2; auto; intros.
-  simpl. rewrite fold_rec_subst_leaf_1; auto.
-  rewrite modify_tree_unroll.
-  destruct p.
-
-  destruct a.
-  rewrite fold_rec_unroll_Some. 
-  rewrite length_fold_rec_split. rewrite IHt2_2.
-  rewrite fold_rec_unroll_Some with (t1:=t2_1) (t2:=t2_2); auto.
-  rewrite length_fold_rec_split with (t2:=t2_2) (acc:=(N.pos (inv_pos n 1)
-       :: fold_rec L.t (list BinNatMap_Base.key)
-            (fun (p0 : BinMap_Base.key) (_ : L.t)
-               (b : list BinNatMap_Base.key) => N.pos p0 :: b) t2_1 n~0 acc)).
-  rewrite plus_Sn_m; auto. 
-  (* dealing with the stupid key *)
-  auto.
-  unfold not; intros; unfold not in H; apply H.
-  clear H.
-(* Lemma random: forall t2 t1 v p,
-  In (N.pos p)
-       (fold L.t (list BinNatMap_Base.key)
-          (fun (p : BinMap_Base.key) (_ : L.t) (b : list BinNatMap_Base.key) =>
-           N.pos p :: b) t2 nil) ->
-  In (N.pos p~1)
-  (fold L.t (list BinNatMap_Base.key)
-     (fun (p0 : BinMap_Base.key) (_ : L.t) (b : list BinNatMap_Base.key) =>
-      N.pos p0 :: b) (node (option L.t) (Some v) t1 t2) nil).
-  Proof.
-    intros t2 t1 v p.
-    rewrite <- ?fold_prop.
-    intro H. apply L3_aux' in H.
-    apply L3_aux.
-    destruct H.
-    exists x. auto.
-    unfold elements. unfold elements in H.
-    simpl.
-    simpl in H.
-    intros; unfold fold; simpl; auto. *)
-    
-
-  unfold fold in H0. 
-  unfold fold. simpl.
-  
-(*   rewrite <- fold_rec_prop  with (l := nil) (b1:=(N.pos (inv_pos 1 1)
-      :: fold_rec L.t (list BinNatMap_Base.key)
-           (fun (p0 : BinMap_Base.key) (_ : L.t) (b : list BinNatMap_Base.key) =>
-            N.pos p0 :: b) t2_1 2 nil)).
-  simpl. admit. *)
-  rewrite <- fold_rec_prop with (l:=nil) (b1:= (N.pos (inv_pos 1 1)
-      :: fold_rec L.t (list BinNatMap_Base.key)
-           (fun (p0 : BinMap_Base.key) (_ : L.t) (b : list BinNatMap_Base.key) =>
-            N.pos p0 :: b) t2_1 2 nil)); auto.
-  apply L3_aux; auto.
-  rewrite <- fold_rec_prop with (l:=nil) (b1:=nil) in H0; auto.
-  simpl.
-  apply L3_aux' in H0. destruct H0.
-  Lemma random : forall p t v,
-    In (p, v) (elements_rec L.t t 1 nil) ->
-    In (p~1, v) (elements_rec L.t t 3 nil).
-  Proof.
-    induction p; induction t; intros; auto.
-    admit. admit.   
-    
-    Lemma L3: forall t p x v, 
-    In (p, v) (elements_rec L.t t x nil) ->
-    In (p~1, v) (elements_rec L.t t x~1 nil).
-  Proof.
-    (* induction x;  *) induction t; intros; simpl; auto.
-    destruct a; auto. simpl. (* simpl in H1. contradiction. *)
-    simpl. (* simpl in H1. destruct o.
-    apply IHx. *)
-(* 
-destruct o. apply IHp in H. 
-    induction t; simpl; intros; auto. *)
-(*       with (acc:=((inv_pos x 1, t) :: elements_rec L.t t1 x~0 acc)); auto. *)
-(*     destruct a. *)
-    simpl.
-    Lemma L4: forall t x k v acc, In (k, v) (elements_rec L.t t x acc) ->
-      In (k, v) (elements_rec L.t t x nil) \/ In (k,v) acc.
-    Proof. induction t; simpl; auto.
-      destruct a.
-      simpl; intros. apply IHt2 in H.
-      inversion H. left. 
-      Lemma L5 : forall t acc x k v, 
-        In (k, v) (elements_rec L.t t x nil) ->
-        In (k, v) (elements_rec L.t t x acc).
-      Proof.
-        induction t as [| a t0 IHt0 t2 IHt2]; simpl in |- *; intros; auto.
-        inversion H.
-        destruct a. apply IHt2; auto. admit.
-        apply IHt2. admit.
-      Admitted.
-      apply L5; auto.
-      inversion H0. rewrite H1. left. 
-        apply in_elements_rec_in_acc. apply in_eq.
-      apply IHt1 in H1.
-      inversion H1. left.  apply in_elements_rec_in_acc. apply in_cons; auto. 
-      right; auto. simpl; intros. apply IHt2 in H.
-      inversion H. left.
-      apply L5; auto.
-      apply IHt1 in H0.
-      inversion H0. left. apply in_elements_rec_in_acc; auto.
-      right; auto.
-    Qed.
-    simpl in H. 
-    apply L4 in H. inversion H.
-    apply IHt2 in H0. admit. 
-    apply in_elements_rec_in_acc; auto. 
-    inversion H0. inversion H1. subst. 
-    assert (forall x, (inv_pos x 1)~1 = inv_pos x 3); auto.
-    clear. intros. induction x; simpl; auto.
-    admit. admit. rewrite H2; apply in_eq.
-    apply in_cons; auto.  apply IHt1 in H1. admit.
-    apply L4 in H. inversion H.
-    apply IHt2 in H0. admit.
-    apply in_elements_rec_in_acc; auto.
-    apply IHt1 in H0.
-    admit.
-  Admitted.
-  exists x.
-  apply L3; auto.
-    apply L4.
-    
-
-      right. inversion H0.
-        unfold not. unfold not in H. intros; apply H. 
-        
-        apply IHacc in H.
-        unfold elements_rec.
-        destruct t. simpl in H. apply in_cons; auto.
-        destruct o. simpl.
-      induction ((inv_pos x 1, t) :: elements_rec L.t t1 x~0 nil); auto.
-      simpl.
-      simpl.
-       
-  admit.
-  admit.
-  destruct a. rewrite fold_rec_unroll_Some. 
-  rewrite length_fold_rec_split. simpl. rewrite IHt2_1.
-  rewrite length_fold_rec_split with (t2:=t2_2) (acc:=(N.pos (inv_pos n 1)
-       :: fold_rec L.t (list BinNatMap_Base.key)
-            (fun (p0 : BinMap_Base.key) (_ : L.t)
-               (b : list BinNatMap_Base.key) => N.pos p0 :: b) t2_1 n~0 acc)).
-  simpl. auto. 
-  unfold not; unfold not in H. intros; apply H. 
-
-  rewrite <- fold_rec_prop with (l:=nil) (b1:= (N.pos (inv_pos 1 1)
-      :: fold_rec L.t (list BinNatMap_Base.key)
-           (fun (p0 : BinMap_Base.key) (_ : L.t) (b : list BinNatMap_Base.key) =>
-            N.pos p0 :: b) t2_1 2 nil)); auto.
-
-    induction acc. inversion H0. contradiction. 
-    destruct a. apply IHt2. 
-    
-    subst; auto.
-    apply IHt2.
-
-    induction t; simpl; intros; auto.
-    admit.
-    destruct a.
-    apply IHt2; auto.
-    destruct (elements_rec L.t t1 x~0 acc).
-    destruct (elements_rec L.t t1 x~1~0 acc). 
-    admit.
-    apply IHt2; auto.
-    elements_rec
-  Admitted. 
-
-  rewrite fold_rec_unroll_None.
-  rewrite length_fold_rec_split. rewrite IHt2_2.
-  rewrite fold_rec_unroll_None.
-  rewrite length_fold_rec_split with (acc:= (fold_rec L.t (list BinNatMap_Base.key)
-         (fun (p0 : BinMap_Base.key) (_ : L.t) (b : list BinNatMap_Base.key)
-          => N.pos p0 :: b) t2_1 n~0 acc)).
-  rewrite plus_Sn_m; auto.
-  unfold not; intros; unfold not in H; apply H.
-  unfold fold in H0.
-  unfold fold.
-  rewrite fold_rec_unroll_None.
-  admit.
-
-  destruct a.
-  rewrite fold_rec_unroll_Some. 
-  rewrite length_fold_rec_split. simpl. rewrite IHt2_1.
-  rewrite length_fold_rec_split with (t2:=t2_2) (acc:=(N.pos (inv_pos n 1)
-       :: fold_rec L.t (list BinNatMap_Base.key)
-            (fun (p0 : BinMap_Base.key) (_ : L.t)
-               (b : list BinNatMap_Base.key) => N.pos p0 :: b) t2_1 n~0 acc)).
-  simpl. omega.
-  (* dealing with the key *)
-  unfold not; intros; unfold not in H; apply H.
-  unfold fold in H0.
-  unfold fold.
-  rewrite fold_rec_unroll_Some.
-  rewrite <- fold_rec_prop  with (l := nil) (b1:=(N.pos (inv_pos 1 1)
-      :: fold_rec L.t (list BinNatMap_Base.key)
-           (fun (p0 : BinMap_Base.key) (_ : L.t) (b : list BinNatMap_Base.key) =>
-            N.pos p0 :: b) t2_1 2 nil)); auto.
-  apply L2_aux. apply in_cons.
-  rewrite <- fold_rec_prop with (l:=nil) (b1:=nil); auto. 
-  rewrite <- fold_rec_prop with (l:=nil) (b1:=nil) in H0; auto.
-(*   destruct t2_1. inversion H0.
-(*   simpl in H0. destruct o. simpl. *)
-(*   apply BinMap.in_fold_cons in H0. *) *)
-  
-    
-  admit.
-
-  rewrite fold_rec_unroll_None.
-  rewrite length_fold_rec_split. simpl. rewrite IHt2_1.
-  rewrite length_fold_rec_split with (acc:= (fold_rec L.t (list BinNatMap_Base.key)
-         (fun (p0 : BinMap_Base.key) (_ : L.t) (b : list BinNatMap_Base.key)
-          => N.pos p0 :: b) t2_1 n~0 acc)).
-  omega.
-  unfold not; intros; unfold not in H; apply H.
-  unfold fold in H0.
-  unfold fold.
-  rewrite fold_rec_unroll_None.
-  rewrite <- fold_rec_prop  with (l := nil) (b1:= fold_rec L.t (list BinNatMap_Base.key)
-           (fun (p0 : BinMap_Base.key) (_ : L.t) (b : list BinNatMap_Base.key) =>
-            N.pos p0 :: b) t2_1 2 nil); auto.
-  apply L2_aux.
-  rewrite <- fold_rec_prop with (l:=nil) (b1:=nil); auto.
-  rewrite <- fold_rec_prop with (l:=nil) (b1:=nil) in H0; auto.
-  apply L3_aux .
-  apply L3_aux' in H0.
-  admit.
-
-  destruct a.
-  apply False_ind.
-  unfold not in H. apply H.
-  apply L1.
-  rewrite ?fold_rec_unroll_Some.
-  rewrite ?fold_rec_unroll_None.
-  rewrite length_fold_rec_split.
-  rewrite length_fold_rec_split with (t2:=t2_2) (acc:= (fold_rec L.t (list BinNatMap_Base.key)
-         (fun (p0 : BinMap_Base.key) (_ : L.t) (b : list BinNatMap_Base.key)
-          => N.pos p0 :: b) t2_1 n~0 acc)).
-  simpl. omega.
-Admitted.  *)
-
-Lemma dom_length_update_nodup : forall m a v, ~In a (VarMap.dom L.t m) ->  
-  length (VarMap.dom L.t (VarMap.update L.t m a v)) = S (length (VarMap.dom L.t m)).
-Proof. 
-  intro m. 
-  destruct m; induction t; auto; intros.
-  destruct o; auto. 
-  destruct a; simpl. contradiction H; simpl; auto.
-  rewrite fold_subst_leaf_1; auto.
-  destruct a; simpl; auto.
-  rewrite fold_subst_leaf_1; auto.
-  (* IH *)
-  (* old proof *)
-  destruct o; destruct a0.
-  contradiction H; simpl; auto.
-  unfold VarMap.dom;
-  unfold BinNatMap_Base.fold;
-  unfold BinMap_Base.fold;
-  unfold VarMap.update; unfold BinNatMap_Base.modify; unfold BinMap_Base.modify.
-  destruct a. 
-  (* case where the fold_rec_unroll_Some *)
-  rewrite modify_tree_unroll.
-  destruct p.
-  (* case of p *)
-  unfold fold.
-  rewrite fold_rec_unroll_Some.
-  rewrite fold_rec_unroll_Some. simpl.
-  rewrite length_fold_rec_split.
-  rewrite length_fold_rec_split with (acc:= (N.pos (inv_pos 1 1)
-         :: fold_rec L.t (list BinNatMap_Base.key)
-              (fun (p0 : BinMap_Base.key) (_ : L.t)
-                 (b : list BinNatMap_Base.key) => N.pos p0 :: b) t1 2 nil)).
-  simpl. rewrite <- plus_Sn_m. 
-  simpl; auto.
-  rewrite length_modify_tree_S; auto.
-  (* case of p~0 *)
-  unfold fold.
-  rewrite ?fold_rec_unroll_Some. simpl.
-  rewrite length_fold_rec_split.
-  rewrite length_fold_rec_split with (acc:=(N.pos (inv_pos 1 1)
-         :: fold_rec L.t (list BinNatMap_Base.key)
-              (fun (p0 : BinMap_Base.key) (_ : L.t)
-                 (b : list BinNatMap_Base.key) => N.pos p0 :: b) t1 2 nil)).
-  simpl. rewrite length_modify_tree_S. omega.
-  (* case of xI *)
-  apply False_ind. 
-  apply H. simpl. right.
-  apply L1.
-  (* case where the fold_rec_unroll_None *)
-  unfold fold;
-  rewrite modify_tree_unroll.
-  destruct p.
-  (* case of p *)
-  rewrite fold_rec_unroll_None.
-  rewrite fold_rec_unroll_None.
-  simpl. rewrite length_fold_rec_split.
-  rewrite length_fold_rec_split with (acc:= (fold_rec L.t (list BinNatMap_Base.key)
-              (fun (p0 : BinMap_Base.key) (_ : L.t)
-                 (b : list BinNatMap_Base.key) => N.pos p0 :: b) t1 2 nil)).
-  simpl. rewrite <- plus_Sn_m.  rewrite length_modify_tree_S; simpl; auto.
-  (* case of p~0 *)
-  rewrite ?fold_rec_unroll_None. simpl.
-  rewrite length_fold_rec_split.
-  rewrite length_fold_rec_split with (acc:=(fold_rec L.t (list BinNatMap_Base.key)
-           (fun (p0 : BinMap_Base.key) (_ : L.t) (b : list BinNatMap_Base.key)
-            => N.pos p0 :: b) t1 2 nil)).
-  rewrite length_modify_tree_S. omega.
-  (* case of xI *)
-  rewrite fold_rec_unroll_Some.
-  rewrite fold_rec_unroll_None. simpl. 
-  rewrite length_fold_rec_split. simpl. rewrite length_fold_rec_split with (acc:=(fold_rec L.t (list BinNatMap_Base.key)
-           (fun (p : BinMap_Base.key) (_ : L.t) (b : list BinNatMap_Base.key)
-            => N.pos p :: b) t1 2 nil)).
-  rewrite <- plus_n_Sm. auto.
-  (* *)
-  simpl; auto.
-  (* *)
-  unfold VarMap.dom;
-  unfold BinNatMap_Base.fold;
-  unfold BinMap_Base.fold;
-  unfold VarMap.update; unfold BinNatMap_Base.modify; unfold BinMap_Base.modify.
-  destruct a. 
-  (* case where the fold_rec_unroll_Some *)
-  rewrite modify_tree_unroll.
-  destruct p.
-  (* case of p *)
-  unfold fold.
-  rewrite ?fold_rec_unroll_Some.
-  rewrite length_fold_rec_split.
-  rewrite length_fold_rec_split with (acc:= (N.pos (inv_pos 1 1)
-         :: fold_rec L.t (list BinNatMap_Base.key)
-              (fun (p0 : BinMap_Base.key) (_ : L.t)
-                 (b : list BinNatMap_Base.key) => N.pos p0 :: b) t1 2 nil)).
-  simpl. rewrite <- plus_Sn_m. apply Nat.add_cancel_r. 
-  rewrite length_modify_tree_S; auto.
-  (* case of p~0 *)
-  unfold fold.
-  rewrite ?fold_rec_unroll_Some.
-  rewrite length_fold_rec_split.
-  rewrite length_fold_rec_split with (acc:=(N.pos (inv_pos 1 1)
-         :: fold_rec L.t (list BinNatMap_Base.key)
-              (fun (p0 : BinMap_Base.key) (_ : L.t)
-                 (b : list BinNatMap_Base.key) => N.pos p0 :: b) t1 2 nil)).
-  simpl. rewrite length_modify_tree_S. omega.
-  (* case of xI *)
-  apply False_ind.
-  apply H. apply L1.
-  (* case where the fold_rec_unroll_None *)
-  rewrite modify_tree_unroll.
-  destruct p.
-  (* case of p *)
-  unfold fold.
-  rewrite ?fold_rec_unroll_None.
-  rewrite length_fold_rec_split.
-  rewrite length_fold_rec_split with (acc:=(fold_rec L.t (list BinNatMap_Base.key)
-           (fun (p0 : BinMap_Base.key) (_ : L.t) (b : list BinNatMap_Base.key)
-            => N.pos p0 :: b) t1 2 nil)).
-  simpl. rewrite <- plus_Sn_m. apply Nat.add_cancel_r.
-  apply length_modify_tree_S.
-  (* case of p~0 *)
-  unfold fold.
-  rewrite ?fold_rec_unroll_None.
-  rewrite length_fold_rec_split.
-  rewrite length_fold_rec_split with (acc:=(fold_rec L.t (list BinNatMap_Base.key)
-           (fun (p0 : BinMap_Base.key) (_ : L.t) (b : list BinNatMap_Base.key)
-            => N.pos p0 :: b) t1 2 nil)).
-  rewrite length_modify_tree_S. omega.
-  (* case of xI *)
-  unfold fold.
-  rewrite fold_rec_unroll_Some.
-  rewrite fold_rec_unroll_None. 
-  rewrite length_fold_rec_split. simpl. rewrite length_fold_rec_split with (acc:=(fold_rec L.t (list BinNatMap_Base.key)
-           (fun (p : BinMap_Base.key) (_ : L.t) (b : list BinNatMap_Base.key)
-            => N.pos p :: b) t1 2 nil)).
-  rewrite plus_n_Sm. auto.
-Qed.
-
-Lemma In_dom_update' : forall a m l v,  ~In a (VarMap.dom L.t m) -> 
-  eq_set (VarMap.dom L.t m) (l) ->
-  eq_set (VarMap.dom L.t (VarMap.update L.t m a v)) (a::l).
+Lemma In_dom_update' : forall a m l v,  ~In a (MapList.dom m) -> 
+  eq_set (MapList.dom m) (l) ->
+  eq_set (@MapList.dom L.t (MapList.update m a v)) (a::l).
   
 Proof.
   split; intros. inversion H0.
@@ -887,62 +289,55 @@ Proof.
   rewrite dom_length_update_nodup; auto. simpl; auto.
   (* dealing with the content *)
   split; intros. auto.
-  apply VarMap.in_dom_get_some in H1.
+  apply MapList.in_dom_get_some in H1.
   generalize (Neq_spec a r); destruct (Neq a r); intros.
   subst; apply in_eq.
-  rewrite VarMap.get_update2 in H1; auto.
-  apply VarMap.get_some_in_dom in H1.
+  rewrite MapList.get_update2 in H1; auto.
+  apply MapList.get_some_in_dom in H1.
   apply in_cons. rewrite H0 in H1; auto.
   generalize (Neq_spec a r); destruct (Neq a r); intros.
-  apply VarMap.get_some_in_dom. subst.
-  rewrite VarMap.get_update1; auto. unfold not; intros. inversion H2.
+  apply MapList.get_some_in_dom. subst.
+  rewrite MapList.get_update1; auto. unfold not; intros. inversion H2.
   inversion H1. apply False_ind; auto.
-  apply VarMap.get_some_in_dom. 
-  rewrite VarMap.get_update2; auto.
-  apply VarMap.in_dom_get_some.
+  apply MapList.get_some_in_dom. 
+  rewrite MapList.get_update2; auto.
+  apply MapList.in_dom_get_some.
   rewrite H0; auto.
 Qed.
 
 Lemma make_rt_from_lvt_prop3 : forall s p v d, NoDup v ->
-  eq_set (VarMap.dom _ (make_rt_from_lvt_rec s p v d)) (v).
+  eq_set (MapList.dom (make_rt_from_lvt_rec s p v d)) (v).
 Proof.
-  intros.
-  induction v; constructor; auto.
-  split; intros H0; inversion H0.
-  assert (make_rt_from_lvt_rec s p (a::v) d = 
-    VarMap.update _ (make_rt_from_lvt_rec s p v d) a (if In_test a p then DEX_lvt s a else d)). auto.
-  rewrite H0. inversion H. apply IHv in H4.
-  inversion H4. inversion H0.
-    rewrite dom_length_update_nodup. simpl; auto.
-    rewrite H4; auto.
-  inversion H. apply IHv in H3.
-  inversion H3; split; intros.
-  assert (make_rt_from_lvt_rec s p (a::v) d = 
-    VarMap.update _ (make_rt_from_lvt_rec s p v d) a (if In_test a p then DEX_lvt s a else d)). auto.
-  generalize (Neq_spec r a); destruct (Neq r a); intros. 
-    subst; apply in_eq.
-    rewrite H7 in H6.
-    apply In_dom_update' with (a:=a) (v:=(if In_test a p then DEX_lvt s a else d)) in H3; auto.
-    inversion H3. apply H10; auto. 
-    (* *)
-    unfold not. intros. rewrite H3 in H9. contradiction.  
-  assert (make_rt_from_lvt_rec s p (a::v) d = 
-    VarMap.update _ (make_rt_from_lvt_rec s p v d) a (if In_test a p then DEX_lvt s a else d)). auto.
-  rewrite H7.
-   apply In_dom_update' with (a:=a) (v:=(if In_test a p then DEX_lvt s a else d)) in H3; auto.
-    inversion H3. apply H9; auto.
-    unfold not; intros. rewrite H3 in H8; contradiction. 
+  induction v; auto; intros.
+  constructor; auto. intros.
+  simpl. split; intros; contradiction.
+  simpl.
+  inversion H. apply IHv with (d:=d) in H3.
+  inversion H3. 
+  constructor. rewrite dom_length_update_nodup; auto. 
+    simpl. rewrite <- H4; auto.
+  rewrite H3; auto.
+  split; intros. 
+  specialize H5 with r. 
+  generalize (Neq_spec r a); destruct (Neq r a); intros.
+  subst. apply in_eq.
+  apply In_dom_update' with (a:=a) (v:=(if In_test a p then DEX_lvt s a else d)) in H3; auto.
+  rewrite <- H3; auto.
+  rewrite H3; auto.
+  apply In_dom_update' with (a:=a) (v:=(if In_test a p then DEX_lvt s a else d)) in H3; auto.
+    inversion H3. apply H8; auto.
+    rewrite H3; auto.
 Qed.
 
-  Definition tsub_rt (rt1 rt2 : VarMap.t L.t) : bool :=
-  (eq_set_test (VarMap.dom _ rt1) (VarMap.dom _ rt2)) &&
-  tsub_rec (rt1) (rt2) (VarMap.dom _ rt2).
+  Definition tsub_rt (rt1 rt2 : MapList.t L.t) : bool :=
+  (eq_set_test (MapList.dom rt1) (MapList.dom rt2)) &&
+  tsub_rec (rt1) (rt2) (MapList.dom rt2).
 
-  Lemma tsub_rec_leq_aux : forall r rt1 rt2, In r (VarMap.dom _ rt2) -> 
-    tsub_rec rt1 rt2 (VarMap.dom _ rt2) = true -> tsub_element rt1 rt2 r = true.
+  Lemma tsub_rec_leq_aux : forall r rt1 rt2, In r (MapList.dom rt2) -> 
+    tsub_rec rt1 rt2 (MapList.dom rt2) = true -> tsub_element rt1 rt2 r = true.
   Proof.
     intros. unfold tsub_rec in H0.
-    induction (VarMap.dom L.t rt2).
+    induction (MapList.dom rt2).
       inversion H.
     elim (andb_prop _ _ H0); intros.
     destruct (reg_eq_dec a r).
@@ -951,10 +346,10 @@ Qed.
     apply IHl in H3; auto.
   Qed.
 
-  Lemma tsub_rec_leq : forall r rt1 rt2 k1 k2, In r (VarMap.dom _ rt2) ->
-    tsub_rec rt1 rt2 (VarMap.dom _ rt2) = true ->
-    Some k1 = VarMap.get _ rt1 r ->
-    Some k2 = VarMap.get _ rt2 r ->
+  Lemma tsub_rec_leq : forall r rt1 rt2 k1 k2, In r (MapList.dom rt2) ->
+    tsub_rec rt1 rt2 (MapList.dom rt2) = true ->
+    Some k1 = MapList.get rt1 r ->
+    Some k2 = MapList.get rt2 r ->
     L.leql k1 k2.
   Proof.
     intros. apply tsub_rec_leq_aux with (rt1:=rt1) in H; auto.
